\documentclass{article}
\usepackage{ifthen}
\usepackage{epsfig}
\usepackage[utf8]{inputenc}
\usepackage{newunicodechar}
  \newunicodechar{⁻}{${}^{-}$}% Superscript minus
  \newunicodechar{²}{${}^{2}$}% Superscript two
  \newunicodechar{³}{${}^{3}$}% Superscript three

\pagestyle{empty}
\begin{document}
$ x = x_m A \sin ( \omega t + \phi )$
\pagebreak

$ x_m, A , \omega t , \phi $
\pagebreak

$x_{t+h} = x_t + h v_{t+h}$
\pagebreak

$v_{t+h} = v_t + h a_{t+h}$
\pagebreak

$v_{t+h} - v_t = dv$
\pagebreak

$ M dv = h f(t+h) $
\pagebreak

$ M dv = h ( f(t) + K dx + (B - r_M M + r_K K) (v+dv) )$
\pagebreak

$ M dv = h ( f(t) + K h (v+dv) + (B - r_M M + r_K K) (v+dv) )$
\pagebreak

$ M $
\pagebreak

$ K = df/dx $
\pagebreak

$ B = df/dv $
\pagebreak

$- r_M M + r_K K$
\pagebreak

$ ( (1+h r_M) M - h B - h(h + r_K) K ) dv = h ( f(t) + (h+r_K) K v + B v - r_M M v )$
\pagebreak

$P$
\pagebreak

$ P ( (1+h r_M) M - h B - h(h + r_K) K ) P dv = P h ( f(t) + (h + r_K) K v + B v - r_M M v )$
\pagebreak

$ M v_t = f_{ext} $
\pagebreak

$ M v_{t+h} = f_{ext_{t+h}} $
\pagebreak

$ = f_{ext_{t}} + h (df_{ext}/dt)_{t+h} $
\pagebreak

$ = f_{ext_{t}} + h (df_{ext}/dx)_{t+h} v_{t+h} $
\pagebreak

$ = f_{ext_{t}} - h K v_{t+h} $
\pagebreak

$ ( M + h K ) v_{t+h} = f_{ext} $
\pagebreak

$v_{t+h} = h/2 ( f(t+h) + f(t) )$
\pagebreak

$ P ( (1+h/2 r_M) M - h/2 B - h/2 (h + r_K) K ) P dv = P h/2 ( 2 f(t) + (h + r_K) K v + B v - r_M M v )$
\pagebreak

$ ( M + h/2 K ) v_{t+h} = f_{ext} $
\pagebreak

\begin{eqnarray*} \vec{R}(\vec{x}) - \vec{P} = 0 \end{eqnarray*}
\pagebreak

$\vec{R}$
\pagebreak

$\vec{P}$
\pagebreak

\begin{align*} \vec{F}(\vec{x}_{n+1}) &= \vec{R}(\vec{x}_{n+1}) - \vec{P}_n \\ \mat{J} = \frac{\partial \vec{F}}{\partial \vec{x}_{n+1}} \bigg\rvert_{\vec{x}_{n+1}^i} &= \mat{K}(\vec{x}_{n+1}) \end{align*}
\pagebreak

$\vec{x}_{n+1}$
\pagebreak

$n$
\pagebreak

\begin{align*} \mat{K}(\vec{x}_{n+1}^i) \left [ \Delta \vec{x}_{n+1}^{i+1} \right ] &= - \vec{F}(\vec{x}_{n+1}^i) \\ \vec{x}_{n+1}^{i+1} &= \vec{x}_{n+1}^{i} + \Delta \vec{x}_{n+1}^{i+1} \end{align*}
\pagebreak

$ \alpha M + \beta B + \gamma C $
\pagebreak

\[ f += B v + K x \]
\pagebreak

\[ df += kFactor K dx + bFactor B dx \]
\pagebreak

\[ df += mFactor M dx + bFactor B dx + kFactor K dx \]
\pagebreak

$ k K $
\pagebreak

$ b B $
\pagebreak

$ m M + b B + k K $
\pagebreak

$ C = K^{-1} $
\pagebreak

\[ res += cFactor C \lambda \]
\pagebreak

$ K $
\pagebreak

$ f += B v + K x $
\pagebreak

$ df += kFactor K dx + bFactor B dx $
\pagebreak

$ kFactor K dx + bFactor B dx $
\pagebreak

$ df = kFactor K dx + bFactor B dx $
\pagebreak

$ res += cFactor * C * lambda $
\pagebreak

$ f_p += dJ^t f_c $
\pagebreak

$ f_p $
\pagebreak

$ f_c $
\pagebreak

$ f(x,v)$
\pagebreak

$ v_c = J v_p $
\pagebreak

$ a_c = J a_p + dJ v_p $
\pagebreak

$ w $
\pagebreak

$ J $
\pagebreak

$ out = J in $
\pagebreak

$ out += J^t in $
\pagebreak

$ \|v\|_l = ( \sum_{i<dim(v)} \|v[i]\|^{l} )^{1/l} $
\pagebreak

$ \|v\|_\infinite = \max_{i<dim(v)} \|v[i]\| $
\pagebreak

$ \begin{array}{ccc} & R & \\ \diagup & & \diagdown \\ A & & B \end{array} $
\pagebreak

$ \begin{array}{ccc} & R & \\ \diagup & & \diagdown \\ A & & B \\ \diagdown & & \diagup \\ & C \end{array} $
\pagebreak

$ u v^T $
\pagebreak

\end{document}
